Enforce safety of proof principles for higher-order store

RGref/DSL/Monad.v
@@ -35,6 +35,45 @@ Axiom rgret : forall {Γ:tyenv}{A:Set}(a:A), rgref Γ A Γ .
 
 Axiom dropvar : forall {Γ} (v:var) (t:Set) (tm:tymember v t Γ), rgref Γ unit (tyrem tm).
 
+(** * Higher-Order Safety *)
+(** The following typeclass network prohibits latent dereference expressions in the heap, alleviating the need for
+    extra caution in proof principles, and removing the need for the type-sensitive semantics in the PLDI'13 paper.
+    It is the subject of a submission to POPL'14. *)
+(* Some background stuff... *)
+  Instance n2n : ImmediateReachability (nat -> nat) := { imm_reachable_from_in := fun _ _ _ _ _ _ => False }.
+  Print Containment.
+  Instance n2nc : Containment (nat -> nat) := {contains := fun _ => False}.
+
+  Instance n2n' : ImmediateReachability (forall x : nat, (fun _ : nat => nat) x) := { imm_reachable_from_in := fun _ _ _ _ _ _ => False }.
+
+
+Class Library {T:Type}(o:T) : Prop := {}.
+Class Safe {T:Type}(t:T) : Prop := {}.
+Class SafeType (T:Type) : Prop := {}.
+Instance safe_lib {T:Type}{o:T}`{Library T o} : Safe o.
+Instance val_of_safe_type {T:Type}`{SafeType T}(t:T) : Safe t.
+Instance imp_of_safe_type {T:Set}`{SafeType T}{Γ}(t : rgref Γ T Γ) : Safe t.
+Instance puretype_safe {T:Set}`{pure_type T} : SafeType T.
+
+Class ESafe (n:nat){T:Type}(t:T) : Prop := { force_proof : False }.
+Instance safe_esafe {T:Type}(t:T){n:nat}`{Safe _ t} : ESafe n t. Admitted.
+Instance esafe_ind {A:Type}{B:A->Type}{n:nat}(f:forall x:A, B x)`{forall a:A, Safe a -> ESafe n (f a)} : ESafe (S n) f.
+Admitted.
+Instance deref_esafe {A B:Set}{P R G}`{rel_fold A}(r:ref{A|P}[R,G]){a b} : ESafe 0 (@deref A B _ P R G a b r).
+Admitted.
+Instance esafe_app {A:Type}{B:A->Type}(f:forall x:A, B x)(a:A){n:nat}`{ESafe (S n) _ f}`{ESafe 0 _ a} : ESafe n (f a).
+Admitted.
+
+Ltac solve_applications :=
+  match goal with
+  | [ |- @ESafe _ _ (?g _ _ _) ] => eapply @esafe_app with (f := g _ _)
+  | [ |- @ESafe _ _ (?g _ _) ] => eapply @esafe_app with (f := g _)
+  | [ |- @ESafe _ _ (?g _) ] => eapply @esafe_app with (f := g)
+  end; eauto with typeclass_instances.
+
+
+
+
 (** The core problem with folding here is that we want the user (and automated provers!) to see the same dereference on either side of
     G's state.  But G applies to elements of A, not [R,G]>>A.  We could introduce an internal "cheat_deref" that skipped
     folding, but then the two sides aren't equal, and many automated tactics that treat !e as essentially an uninterpreted
@@ -63,7 +102,7 @@ Axiom dropvar : forall {Γ} (v:var) (t:Set) (tm:tymember v t Γ), rgref Γ unit 
                    G (!l) e h (heap_write l e h)}
                  {pres:(forall h (l:ref{A|P}[R,G]), P (!l) h -> P e (heap_write l e h))}
                  , rgref Γ unit Γ.*)
-Program Axiom write' : forall {Γ:tyenv}{A:Set}`{rel_fold A}{P R G}`{hreflexive G}(x:ref{A|P}[R,G])(e:A)
+Program Axiom write' : forall {Γ:tyenv}{A:Set}`{rel_fold A}{P R G}`{hreflexive G}(x:ref{A|P}[R,G])(e:A)`{ESafe 0 A e}
                       (meta_x_deref:A) (meta_e_fold:A) 
                       (** These meta args are notationally expanded x and e using the identity relation folding *)
                  (*{guar:forall h, G (!x) e h (heap_write x e h)} *)
@@ -71,7 +110,7 @@ Program Axiom write' : forall {Γ:tyenv}{A:Set}`{rel_fold A}{P R G}`{hreflexive 
                  (** temporarily not using meta_e_fold... the cases where I needed the "nop" behavior are once where the types are actually equal *)
                  {pres:(forall h, P meta_x_deref h -> P meta_e_fold (heap_write x meta_e_fold h))}
                  , rgref Γ unit Γ.
-Notation "[ x ]:= e" := (@write' _ _ _ _ _ _ _ x e ({{{!x}}}) ({{{e}}}) _ _) (at level 70).
+Notation "[ x ]:= e" := (@write' _ _ _ _ _ _ _ x e _ ({{{!x}}}) ({{{e}}}) _ _) (at level 70).
 (** TODO: heap writes that update the predicate.  Because of the monadic style, we'll actually
    need a new axiom and syntax support for this, to rebind the variable at the strengthened type *)
 
@@ -99,6 +138,7 @@ Program Axiom read_imp : forall {Γ}{A B:Set}`{rel_fold A}{P R G}`{hreflexive G}
 
 (* Writing with an impure source expression (and direct ref value) *)
 Program Axiom write_imp_exp : forall {Γ Γ'}{A:Set}`{rel_fold A}{P R G}`{hreflexive G}(x:ref{A|P}[R,G])(e:rgref Γ A Γ')
+                              `{ESafe 0 _ e}
                               (meta_x_deref:rgref Γ A Γ') (meta_e_fold:rgref Γ A Γ')
                               {guar:forall h env, G (valueOf _ _ _ env h meta_x_deref) (valueOf _ _ _ env h e) h (heap_write x (valueOf _ _ _ env h e) h)}
                               {pres:(forall h env, P (valueOf _ _ _ env h meta_x_deref) h -> P (valueOf _ _ _ env h meta_e_fold) (heap_write x (valueOf _ _ _ env h meta_e_fold) h))}
@@ -109,36 +149,39 @@ Definition locally_const {A:Set} (R:hrel A) := forall a a' h h', R a a' h h' -> 
 
 
 Axiom alloc : forall {Γ}{T:Set}{RT:ImmediateReachability T}{CT:Containment T}{FT:rel_fold T} P R G (e:T), 
+                ESafe 0 e ->
                 stable P R ->        (* predicate is stable *)
                 (forall h, P e h) -> (* predicate is true *)
                 precise_pred P ->    (* P precise *)
                 precise_rel R ->     (* R precise *)
                 precise_rel G ->     (* G precise *)
                 rgref Γ (ref{T|P}[R,G]) Γ.
-Notation "'Alloc' e" := (alloc _ _ _ e _ _ _ _ _) (at level 70).
+Notation "'Alloc' e" := (alloc _ _ _ e _ _ _ _ _ _) (at level 70).
 (** Sometimes it is useful to refine P to give equality with the allocated value, which
     propagates assumptions and equalities across "statements." *)
 Axiom alloc' : forall {Γ}{T:Set}{RT:ImmediateReachability T}{CT:Containment T}{FT:rel_fold T} P R G (e:T) (meta_e:T),
+                ESafe 0 e ->
                 stable P R ->        (* predicate is stable *)
                 (forall h, P e h) -> (* predicate is true *)
                 precise_pred P ->    (* P precise *)
                 precise_rel R ->     (* R precise *)
                 precise_rel G ->     (* G precise *)
                  rgref Γ (ref{T|P ⊓ (fun t=>fun h=> (locally_const R -> t=meta_e))}[R,G]) Γ.
-Notation "Alloc! e" := (alloc' _ _ _ e ({{{e}}}) _ _ _ _ _) (at level 70).
+Notation "Alloc! e" := (alloc' _ _ _ e ({{{e}}}) _ _ _ _ _ _) (at level 70).
                                  
 
   
 Notation "x <- M ; N" := (rgref_bind M (fun x => N)) (at level 49, right associativity).
 
 Axiom varalloc' : forall {Γ}{T:Set}{RT:ImmediateReachability T}{CT:Containment T}{FT:rel_fold T} P R G (v:var) (e:T) (meta_e:T),
+                ESafe 0 e ->
                 stable P R ->        (* predicate is stable *)
                 (forall h, P e h) -> (* predicate is true *)
                 precise_pred P ->    (* P precise *)
                 precise_rel R ->     (* R precise *)
                 precise_rel G ->     (* G precise *)
                  rgref Γ unit (v:ref{T|P ⊓ (fun t=>fun h=> (locally_const R -> t=meta_e))}[R,G],Γ).
-Notation "VarAlloc! v e" := (varalloc' _ _ _ v e ({{{e}}}) _ _ _ _ _) (at level 70).
+Notation "VarAlloc! v e" := (varalloc' _ _ _ v e ({{{e}}}) _ _ _ _ _ _) (at level 70).
 
 
 
