MemoTable.v
@@ -1,0 +1,58 @@
+Require Import RGref.DSL.DSL.
+Require Import Coq.Arith.Arith.
+
+Section MemoTable.
+
+  (* Apparently the instances below stick around after the section ends... *)
+  Variable B : nat -> Set.
+  Variable f : forall (x:nat), B x.
+  Parameter safe_f : Safe f.
+  Existing Instance safe_f.
+  Parameter safe_B : Safe B.
+  Existing Instance safe_B.
+
+  Definition prefernat {P:nat->Set}(g:forall x:nat, P x)(a:nat) : forall x:nat, P x.
+    refine(let v := g a in
+             (fun x => if eq_nat_dec x a then _ else g x)).
+    subst. exact v.
+  Defined.
+  Print prefernat.
+
+  Definition obs_equiv {A:Set}{P:A->Set}(f g:forall x, P x)(_ _:heap) :=
+    forall x, f x = g x.
+  Lemma obs_eq_refl : forall A P, hreflexive (@obs_equiv A P).
+  Proof. intros; red. compute. eauto. Qed.
+  Hint Resolve obs_eq_refl.
+  Lemma precise_obs_equiv : precise_rel (@obs_equiv nat (fun _ => nat)).
+  Proof. compute. intuition. Qed.
+  Hint Resolve precise_obs_equiv.
+
+  Instance safe_prefernat : Safe (@prefernat).
+(*  Instance prior_safe (r:ref{forall x:nat,B x|any}[obs_equiv,obs_equiv]) (n:nat)
+    : Safe (@prefernat B (@deref _ _ _ _ _ _ (obs_eq_refl _ _) eq_refl r) n). *)
+  Instance prior_safe (r:ref{forall x:nat,B x|any}[obs_equiv,obs_equiv]) (n:nat)
+                              : ESafe 0 (@prefernat B f n).
+    repeat solve_applications.
+  Defined.
+    
+  Program Definition prioritize {Γ} (r:ref{forall x:nat,B x|any}[obs_equiv,obs_equiv]) (n:nat) : rgref Γ unit Γ :=
+    [r]:= prefernat (!r) n.
+  Next Obligation.
+    repeat solve_applications.
+  Qed.
+  Next Obligation.
+    red. unfold prefernat. intros. induction (eq_nat_dec x n); intuition; eauto.
+    subst. compute. eauto.
+  Qed.
+(* Doesn't (and shouldn't!) typecheck *)
+  Program Example should_not_typecheck {Γ} (r:ref{nat|any}[havoc,havoc]) : rgref Γ (ref{nat->nat|any}[havoc,havoc]) Γ :=
+    Alloc (fun x => !r). (*;
+    prioritize _ r 0.
+  (*Print should_not_typecheck.*)
+*)
+  Next Obligation. compute; eauto. Defined.
+  Next Obligation.
+    (* Cannot typecheck because (λ x:N. !r) is in fact not safe! *)
+  Admitted.
+
+End MemoTable.
